Wavelet/Determinacy/PCM.lean
@@ -1,3 +1,5 @@
+import Mathlib.Data.List.Basic
+
 /-! Definitions for PCM. -/
 
 namespace Wavelet.Determinacy
@@ -35,6 +37,22 @@ class Lawful (R : Type u) [inst : PCM R] where
   add_ident : ∀ {a : R}, a ⊔ inst.zero = a
   valid_add : ∀ {a b : R}, ✓ a ⊔ b → ✓ a
   valid_zero : ✓ inst.zero
+
+instance [inst : PCM R] [Lawful R] : Std.Commutative inst.add where
+  comm := by apply Lawful.add_comm
+
+instance [inst : PCM R] [Lawful R] : Std.Associative inst.add where
+  assoc := by apply Lawful.add_assoc
+
+instance [inst : PCM R] : Std.LeftIdentity inst.add inst.zero where
+
+instance [inst : PCM R] [Lawful R] : Std.LawfulLeftIdentity inst.add inst.zero where
+  left_id a := by rw [Lawful.add_comm]; apply Lawful.add_ident
+
+instance [inst : PCM R] : Std.RightIdentity inst.add inst.zero where
+
+instance [inst : PCM R] [Lawful R] : Std.LawfulRightIdentity inst.add inst.zero where
+  right_id a := by apply Lawful.add_ident
 
 class Cancellative (R : Type u) [PCM R] where
   cancel_left : ∀ {a b c : R}, a ⊔ b = a ⊔ c → b = c
@@ -74,6 +92,142 @@ theorem valid.add_right [PCM C] [Lawful C] {a b : C} (h : ✓ a ⊔ b) : ✓ b
   := by
   rw [Lawful.add_comm] at h
   exact Lawful.valid_add h
+
+theorem valid.le [PCM C] [Lawful C] {a b : C} (h : ✓ b) (hle : a ≤ b) : ✓ a := by
+  have ⟨c, h⟩ := hle
+  subst h
+  apply valid.add_left h
+
+theorem framePreserving.from_le [PCM C] [Lawful C]
+  {a b : C} (hle : a ≤ b) : b ⟹ a := by
+  have ⟨c, h⟩ := hle
+  subst h
+  intros d hd
+  rw [Lawful.add_comm, ← Lawful.add_assoc] at hd
+  have := hd.add_left
+  rw [Lawful.add_comm] at this
+  exact this
+
+theorem framePreserving.congr_add_left [PCM C] [Lawful C]
+  {a b c : C} (hfp : a ⟹ b) : c ⊔ a ⟹ c ⊔ b := by
+  intros d hd
+  rw [Lawful.add_assoc, Lawful.add_comm, Lawful.add_assoc] at hd ⊢
+  apply hfp _ hd
+
+@[simp]
+theorem add.right_zero_id [PCM C] [Lawful C] (a : C) : a ⊔ PCM.zero = a :=
+  Lawful.add_ident
+
+@[simp]
+theorem add.left_zero_id [PCM C] [Lawful C] (a : C) : PCM.zero ⊔ a = a := by
+  rw [Lawful.add_comm]; apply Lawful.add_ident
+
+@[simp]
+theorem add.le_add_right [PCM C] {a b : C} : a ≤ a ⊔ b := by exists b
+
+theorem add.le_add_right_alt [PCM C] [PCM.Lawful C] {a b c : C} (h : a ≤ b) : a ≤ c ⊔ b := by
+  have ⟨d, hd⟩ := h
+  subst hd
+  rw [Lawful.add_comm, Lawful.add_assoc]
+  simp
+
+@[simp]
+theorem add.le_add_left [PCM C] [PCM.Lawful C] {a b : C} : b ≤ a ⊔ b := by
+  rw [Lawful.add_comm];
+  exists a
+
+theorem add.le_add_left_alt [PCM C] [PCM.Lawful C] {a b c : C} (h : a ≤ b) : a ≤ b ⊔ c := by
+  have ⟨d, hd⟩ := h
+  subst hd
+  rw [Lawful.add_assoc]
+  simp
+
+theorem add.le_add_congr [PCM C] [PCM.Lawful C]
+  {a₁ a₂ b₁ b₂ : C} (ha : a₁ ≤ a₂) (hb : b₁ ≤ b₂) :
+    a₁ ⊔ b₁ ≤ a₂ ⊔ b₂ := by
+  have ⟨c₁, hc₁⟩ := ha
+  have ⟨c₂, hc₂⟩ := hb
+  subst hc₁; subst hc₂
+  calc
+    a₁ ⊔ b₁ ≤ (a₁ ⊔ b₁) ⊔ (c₁ ⊔ c₂) := by simp
+    _ = _  := by
+      rw [Lawful.add_assoc, Lawful.add_assoc]
+      rw [@Lawful.add_comm _ _ _ b₁ (c₁ ⊔ c₂)]
+      rw [@Lawful.add_assoc]
+      rw [@Lawful.add_comm _ _ _ b₁ c₂]
+
+@[simp]
+theorem le.refl [PCM C] [Lawful C] (a : C) : a ≤ a := by exists PCM.zero; simp
+
+@[simp]
+theorem sum.nil [inst : PCM C] : sum [] = inst.zero := by simp [sum]
+
+@[simp]
+theorem sum.singleton [PCM C] [Lawful C] (a : C) : sum [a] = a := by
+  simp [sum, Lawful.add_comm]
+
+@[simp]
+theorem sum.cons [PCM C] [Lawful C] (a : C) (xs : List C) : sum (a :: xs) = a ⊔ sum xs := by
+  induction xs generalizing a with
+  | nil => simp
+  | cons x xs ih =>
+    rw [ih, sum]
+    simp [List.foldl_eq_foldr]
+    rw [sum]
+    simp [List.foldl_eq_foldr]
+
+@[simp]
+theorem sum.append [PCM C] [Lawful C] (xs ys : List C) :
+  sum (xs ++ ys) = sum xs ⊔ sum ys := by
+  induction xs with
+  | nil => simp [Lawful.add_comm]
+  | cons a xs ih =>
+    simp [ih]
+    rw [Lawful.add_assoc]
+
+theorem sum.mem_to_le [PCM C] [Lawful C] {xs : List C}
+  {a : C} (hmem : a ∈ xs) :
+  a ≤ sum xs := by
+  induction xs with
+  | nil => simp at hmem
+  | cons x xs ih =>
+    simp at hmem
+    cases hmem with
+    | inl h₁ => subst h₁; simp
+    | inr h₁ =>
+      specialize ih h₁
+      simp [add.le_add_right_alt ih]
+
+theorem sum.le_disj_get [PCM C] [Lawful C] {xs : List C}
+  (hne : i ≠ j)
+  (hi : i < xs.length)
+  (hj : j < xs.length) :
+    xs[i] ⊔ xs[j] ≤ sum xs := by
+  induction xs generalizing i j with
+  | nil => simp at hi
+  | cons x xs ih =>
+    simp at hi hj
+    cases i with
+    | zero =>
+      cases j with
+      | zero => contradiction
+      | succ j' =>
+        simp
+        apply add.le_add_congr
+        · simp
+        · apply sum.mem_to_le; simp
+    | succ i' =>
+      cases j with
+      | zero =>
+        simp
+        rw [Lawful.add_comm]
+        apply add.le_add_congr
+        · simp
+        · apply sum.mem_to_le; simp
+      | succ j' =>
+        simp at hne ⊢
+        apply add.le_add_right_alt
+        apply ih hne
 
 end PCM
 
